src/Language.v
@@ -1,43 +1,46 @@
 (* Celsius project *)
-(* Clément Blaudeau - Lamp@EPFL 2021 *)
-(** This file defines all the basic structures (as inductive types) of the project. *)
+(* Clément Blaudeau - Lamp@EPFL & Inria 2020-2022 *)
+
+(** This file defines all the basic structures of the language (as inductive types). *)
+
+From Celsius Require Export Tactics.
 Require Import Coq.Lists.List Psatz Ensembles.
 Import ListNotations.
-From Celsius Require Export Tactics.
 
 (** * Language structures *)
 
 (** ** Basic types *)
 Definition Var : Type := nat.
-Definition Mtd : Type := nat.
+Variant Mtd : Type := mtd(n: nat).
 Definition Loc : Type := nat.
 Variant ClN : Type := cln(n: nat).
 
-
 (** ** Expression constructors *)
 Inductive Expr: Type :=
-| var   : Var -> Expr
-| this
-| fld   : Expr -> Var -> Expr
-| mtd   : Expr -> Mtd -> (list Expr) -> Expr
-| new   : ClN -> (list Expr) -> Expr
-| asgn  : Expr -> Var -> Expr -> Expr -> Expr.
+| e_var   : Var -> Expr
+| e_this
+| e_fld   : Expr -> Var -> Expr
+| e_mtd   : Expr -> Mtd -> (list Expr) -> Expr
+| e_new   : ClN -> (list Expr) -> Expr
+| e_asgn  : Expr -> Var -> Expr -> Expr -> Expr.
 
+(** ** Modes *)
 Inductive Mode: Type :=
 | hot
 | warm
 | cool : nat -> Mode
 | cold.
 
+(** ** Types *)
 Notation "'Tpe'" := (prod ClN Mode).
 
+(** ** Other language constructions *)
 Variant Field   : Type := field(type: Tpe)(expr: Expr).
 Variant Method  : Type := method(μ: Mode)(args: list Tpe)(out_type: Tpe)(body: Expr).
 Variant Class   : Type := class(args: list Tpe)(fields: list Field)(methods: Mtd -> (option Method)).
 Variant Program : Type := program(C: list Class)(entry: Expr).
 
-
-(** ** Constructs *)
+(** ** Other Types *)
 Definition Value : Type := Loc.
 Definition Env: Type   := list Value.
 Definition EnvTyping: Type := list Tpe.
@@ -54,4 +57,4 @@ Parameter EntryClass: Class.
 
 Definition ct (C:ClN) := match C with | cln n => nth n Ξ EntryClass end.
 Parameter EntryClass_ct : ct Entry = EntryClass.
-Definition main: Mtd := 0.
+Definition main: Mtd := mtd(0).
