src/Semantics.v
@@ -4,62 +4,62 @@
 
 From Celsius Require Export Language Notations Helpers LibTactics .
 Require Import ssreflect ssrbool  Coq.Program.Tactics.
-Import List Psatz Arith.
-Import ListNotations.
+Import List Psatz Arith ListNotations.
 Open Scope nat_scope.
 
 (* Notation only used for the definition *)
 Reserved Notation "'⟦'  e  '⟧p' '(' σ ',' ρ ',' v ')'  '-->'  '(' v0 ',' σ0 ')'" (at level 80).
 Reserved Notation "'⟦_' e '_⟧p' '(' σ ',' ρ ',' v ')'  '-->'  '(' vl ',' σl ')'" (at level 80).
+
 Inductive evalP : Expr -> Store -> Env -> Value -> Value -> Store -> Prop :=
 
 (** variable *)
-| e_var : forall σ x ρ ψ l,
+| bs_var : forall σ x ρ ψ l,
     getVal ρ x = Some l ->
-    ⟦ var x ⟧p (σ, ρ, ψ) --> (l, σ)
+    ⟦ e_var x ⟧p (σ, ρ, ψ) --> (l, σ)
 
 (** this *)
-| e_this : forall σ ρ ψ,
-    ⟦ this ⟧p (σ, ρ, ψ) --> (ψ, σ)
+| bs_this : forall σ ρ ψ,
+    ⟦ e_this ⟧p (σ, ρ, ψ) --> (ψ, σ)
 
 (** field access *)
-| e_fld : forall σ ρ ψ e f v1 σ1 C ω v,
+| bs_fld : forall σ ρ ψ e f v1 σ1 C ω v,
     ⟦ e ⟧p (σ, ρ, ψ) --> (v1, σ1) ->
     getObj σ1 v1 = Some (C, ω) ->
     getVal ω f = Some v ->
-    ⟦ (fld e f) ⟧p (σ, ρ, ψ) --> (v, σ1)
+    ⟦ (e_fld e f) ⟧p (σ, ρ, ψ) --> (v, σ1)
 
 (** method call : e0.m(args) *)
-| e_mtd : forall σ e0 m el e2 ρ ψ l1 vl2 l3 σ1 σ2 σ3 C Args Flds Mtds f argsM T μ,
+| bs_mtd : forall σ e0 m el e2 ρ ψ l1 vl2 l3 σ1 σ2 σ3 C Args Flds Mtds f argsM T μ,
     ⟦ e0 ⟧p (σ, ρ, ψ) --> (l1, σ1) ->
     getObj σ1 l1 = Some (C, f) ->
     ⟦_ el _⟧p (σ1, ρ, ψ) --> (vl2, σ2) ->
     ct C = class Args Flds Mtds  ->
     Mtds m = Some (method μ argsM T e2) ->
     ⟦ e2 ⟧p (σ2, vl2, l1) --> (l3, σ3) ->
-    ⟦ mtd e0 m el ⟧p (σ, ρ, ψ) --> (l3, σ3)
+    ⟦ e_mtd e0 m el ⟧p (σ, ρ, ψ) --> (l3, σ3)
 
 (** new class *)
-| e_new : forall σ ρ ψ C Args Flds Mtds args vl__args σ1 σ3,
+| bs_new : forall σ ρ ψ C Args Flds Mtds args vl__args σ1 σ3,
     ⟦_ args _⟧p (σ, ρ, ψ) --> (vl__args, σ1) ->
     ct C = class Args Flds Mtds ->
     let I := (length σ1) in
     initP C I 0 vl__args (σ1 ++ [(C, [])]) σ3 ->
-    ⟦ new C args ⟧p (σ, ρ, ψ) --> (I, σ3)
+    ⟦ e_new C args ⟧p (σ, ρ, ψ) --> (I, σ3)
 
 (** assignment *)
-| e_asgn : forall σ ρ ψ e1 x e2 e' σ1 v1 σ2 v2 σ3 v3,
+| bs_asgn : forall σ ρ ψ e1 x e2 e' σ1 v1 σ2 v2 σ3 v3,
     ⟦ e1 ⟧p (σ, ρ, ψ) --> (v1, σ1) ->
     ⟦ e2 ⟧p (σ1, ρ, ψ) --> (v2, σ2) ->
     ⟦ e' ⟧p ((assign v1 x v2 σ2), ρ, ψ) --> (v3, σ3) ->
-    ⟦ asgn e1 x e2 e' ⟧p (σ, ρ, ψ) --> (v3, σ3)
+    ⟦ e_asgn e1 x e2 e' ⟧p (σ, ρ, ψ) --> (v3, σ3)
 
 where "'⟦' e '⟧p' '(' σ ',' ρ ',' v ')' '-->' '(' v0 ',' σ0 ')' "  := (evalP e σ ρ v v0 σ0)
 
 with evalListP : list Expr -> Store -> Env -> Value -> list Value -> Store -> Prop :=
-| el_nil : forall σ ρ ψ,
+| bs_nil : forall σ ρ ψ,
     ⟦_ [] _⟧p (σ, ρ, ψ) --> ([], σ)
-| el_cons : forall σ ρ ψ e el l1 σ1 vl σ2,
+| bs_cons : forall σ ρ ψ e el l1 σ1 vl σ2,
     ⟦ e ⟧p (σ, ρ, ψ) --> (l1, σ1) ->
     ⟦_ el _⟧p (σ1, ρ, ψ) --> (vl, σ2) ->
     ⟦_ (e::el) _⟧p (σ, ρ, ψ) --> (l1::vl, σ2)
@@ -93,38 +93,38 @@ Section evalP_ind.
   Variable Pin : forall C ψ x ρ σ σ', (initP C ψ x ρ σ σ') -> Prop.
 
   Variable P_var : forall σ x ρ ψ l Hget,
-      P (var x) σ ρ ψ l σ (e_var σ x ρ ψ l Hget).
+      P (e_var x) σ ρ ψ l σ (bs_var σ x ρ ψ l Hget).
 
   Variable P_this : forall σ ρ ψ,
-      P this σ ρ ψ ψ σ (e_this σ ρ ψ).
+      P e_this σ ρ ψ ψ σ (bs_this σ ρ ψ).
 
   Variable P_fld : forall σ ρ ψ e f v1 σ1 C ω v EH__e0 H__getObj H__getVal
     (IH__e0: P e σ ρ ψ v1 σ1 (EH__e0)),
-    P (fld e f) σ ρ ψ v σ1 (e_fld σ ρ ψ e f v1 σ1 C ω v EH__e0 H__getObj H__getVal).
+    P (e_fld e f) σ ρ ψ v σ1 (bs_fld σ ρ ψ e f v1 σ1 C ω v EH__e0 H__getObj H__getVal).
 
   Variable P_mtd : forall σ e0 m el e2 ρ ψ v1 vl2 v3 σ1 σ2 σ3 C f argsC argsM fields methods T μ H__e0 Hobj H__el Hct Hmth  H__e2
     (IH__e0: P e0 σ ρ ψ v1 σ1 H__e0)
     (IH__el: Pl el σ1 ρ ψ vl2 σ2 H__el)
     (IH__e2: P e2 σ2 vl2 v1 v3 σ3 H__e2),
-    P( mtd e0 m el) σ ρ ψ v3 σ3 (e_mtd σ e0 m el e2 ρ ψ v1 vl2 v3 σ1 σ2 σ3 C f argsC argsM fields methods T μ H__e0 Hobj H__el Hct Hmth H__e2).
+    P( e_mtd e0 m el) σ ρ ψ v3 σ3 (bs_mtd σ e0 m el e2 ρ ψ v1 vl2 v3 σ1 σ2 σ3 C f argsC argsM fields methods T μ H__e0 Hobj H__el Hct Hmth H__e2).
 
   Variable P_new : forall σ ρ ψ C args vl__args σ1 σ3 Args Flds Mtds H__args H__ct H__init
     (IH__args: Pl args σ ρ ψ vl__args σ1 H__args)
     (IH__init: Pin C (length σ1) 0 vl__args (σ1 ++ [(C, [])]) σ3 H__init),
-    P (new C args) σ ρ ψ (length σ1) σ3 (e_new σ ρ ψ C Args Flds Mtds args vl__args σ1 σ3 H__args H__ct H__init).
+    P (e_new C args) σ ρ ψ (length σ1) σ3 (bs_new σ ρ ψ C Args Flds Mtds args vl__args σ1 σ3 H__args H__ct H__init).
 
   Variable P_asgn :  forall σ ρ ψ e1 x e2 e' σ1 v1 σ2 v2 σ3 v3 H__e1 H__e2 H__e'
     (IH__e1: P e1 σ ρ ψ v1 σ1 H__e1)
     (IH__e2: P e2 σ1 ρ ψ v2 σ2 H__e2)
     (IH__e': P e' (assign v1 x v2 σ2) ρ ψ v3 σ3 H__e'),
-    P (asgn e1 x e2 e') σ ρ ψ v3 σ3 (e_asgn σ ρ ψ e1 x e2 e' σ1 v1 σ2 v2 σ3 v3 H__e1 H__e2 H__e').
+    P (e_asgn e1 x e2 e') σ ρ ψ v3 σ3 (bs_asgn σ ρ ψ e1 x e2 e' σ1 v1 σ2 v2 σ3 v3 H__e1 H__e2 H__e').
 
-  Variable Pl_nil : forall σ ρ ψ, Pl [] σ ρ ψ [] σ (el_nil σ ρ ψ).
+  Variable Pl_nil : forall σ ρ ψ, Pl [] σ ρ ψ [] σ (bs_nil σ ρ ψ).
 
   Variable Pl_cons : forall σ ρ ψ e el v1 σ1 vl σ2 H__e H__el
       (IH__e: P e σ ρ ψ v1 σ1 H__e)
       (IH__el: Pl el σ1 ρ ψ vl σ2 H__el),
-      Pl (e::el) σ ρ ψ (v1::vl) σ2 (el_cons σ ρ ψ e el v1 σ1 vl σ2 H__e H__el).
+      Pl (e::el) σ ρ ψ (v1::vl) σ2 (bs_cons σ ρ ψ e el v1 σ1 vl σ2 H__e H__el).
 
   Variable Pin_nil: forall C I ρ σ Args Flds Mtds H__ct,
       Pin C I (length Flds) ρ σ σ (init_nil C I ρ σ Args Flds Mtds H__ct).
@@ -136,20 +136,20 @@ Section evalP_ind.
 
   Fixpoint evalP_ind2 e σ ρ ψ v σ' (eval : evalP e σ ρ ψ v σ') : P e σ ρ ψ v σ' eval :=
     match eval with
-    | e_var σ x ρ ψ v Hget => P_var σ x ρ ψ v Hget
-    | e_this σ ρ ψ => P_this σ ρ ψ
-    | e_fld σ ρ ψ e0 x l1 σ1 C f v1 H__e0 Hobj Hval =>
+    | bs_var σ x ρ ψ v Hget => P_var σ x ρ ψ v Hget
+    | bs_this σ ρ ψ => P_this σ ρ ψ
+    | bs_fld σ ρ ψ e0 x l1 σ1 C f v1 H__e0 Hobj Hval =>
         P_fld σ ρ ψ e0 x l1 σ1 C f v1 H__e0 Hobj Hval (evalP_ind2 e0 σ ρ ψ l1 σ1 H__e0)
-    | e_mtd σ e0 m el e2 ρ ψ l1 vl2 l3 σ1 σ2 σ3 C f argsC argsM fields methods T μ H__e0 Hobj H__el Hct Hmth H__e2 =>
+    | bs_mtd σ e0 m el e2 ρ ψ l1 vl2 l3 σ1 σ2 σ3 C f argsC argsM fields methods T μ H__e0 Hobj H__el Hct Hmth H__e2 =>
         P_mtd σ e0 m el e2 ρ ψ l1 vl2 l3 σ1 σ2 σ3 C f argsC argsM fields methods T μ H__e0 Hobj H__el Hct Hmth H__e2
               (evalP_ind2 e0 σ ρ ψ l1 σ1 H__e0)
               (evalListP_ind2 el σ1 ρ ψ vl2 σ2 H__el)
               (evalP_ind2 e2 σ2 vl2 l1 l3 σ3 H__e2)
-    | e_new σ ρ ψ C Args Flds Mtds args vl__args σ1 σ3 H__args H__ct H__init =>
+    | bs_new σ ρ ψ C Args Flds Mtds args vl__args σ1 σ3 H__args H__ct H__init =>
         P_new σ ρ ψ C args vl__args σ1 σ3 Args Flds Mtds H__args H__ct H__init
               (evalListP_ind2 args σ ρ ψ vl__args σ1 H__args)
               (initP_ind2 C (length σ1) 0 vl__args (σ1 ++ [(C, [])]) σ3 H__init)
-    | e_asgn σ ρ ψ e1 x e2 e' σ1 v1 σ2 v2 σ3 v3 H__e1 H__e2 H__e' =>
+    | bs_asgn σ ρ ψ e1 x e2 e' σ1 v1 σ2 v2 σ3 v3 H__e1 H__e2 H__e' =>
         P_asgn σ ρ ψ e1 x e2 e' σ1 v1 σ2 v2 σ3 v3 H__e1 H__e2 H__e'
                (evalP_ind2 e1 σ ρ ψ v1 σ1 H__e1)
                (evalP_ind2 e2 σ1 ρ ψ v2 σ2 H__e2)
@@ -158,8 +158,8 @@ Section evalP_ind.
 
   with evalListP_ind2 el σ ρ ψ vl σ' evalList : Pl el σ ρ ψ vl σ' evalList :=
          match evalList  with
-         | el_nil σ ρ ψ  => Pl_nil σ ρ ψ
-         | el_cons σ ρ ψ e el l1 σ1 vl σ2 H__e H__el =>
+         | bs_nil σ ρ ψ  => Pl_nil σ ρ ψ
+         | bs_cons σ ρ ψ e el l1 σ1 vl σ2 H__e H__el =>
              Pl_cons σ ρ ψ e el l1 σ1 vl σ2 H__e H__el
                      (evalP_ind2 e σ ρ ψ l1 σ1 H__e)
                      (evalListP_ind2 el σ1 ρ ψ vl σ2 H__el)
